pulse/src/checker/Pulse.Reflection.Util.fst
@@ -311,6 +311,7 @@ let non_informative_witness_rt (u:R.universe) (a:R.term) : R.term =
 
 let unit_non_informative_lid = mk_pulse_lib_core_lid "unit_non_informative"
 let prop_non_informative_lid = mk_pulse_lib_core_lid "prop_non_informative"
+let erased_non_informative_lid = mk_pulse_lib_core_lid "erased_non_informative"
 let squash_non_informative_lid = mk_pulse_lib_core_lid "squash_non_informative"
 
 let stt_vprop_equiv_fv =
